# Differential Forms

```{definition, , name="Differential"}

If $f \in C^\infty_p(M)$, then its differential at $p$ is defined to be the covector $df \in T_pM^\vee$ such that
$$
(df)_p(X) = X(f)
$$

```

```{theorem}

At any point $p \in M$, if $(U, x^1, \dots, x^n)$ is a chart about $p$, then the differentials
$$
dx^1, \quad \dots, \quad dx^n
$$
comprise a basis for $T_pM^\vee$ such that
$$
df = \sum \frac{\partial f}{\partial x^i} dx^i
$$
for any $f \in C_p^\infty(M)$

```



## Exterior Power of Cotangent Bundle

```{definition, , name="Cotangent Bundle"}

The cotangent bundle of a manifold $M$ is denoted by $T^*M$, defined in similar fashion of tangent bundle.

```

```{definition, , name="Alternating tensor"}

A $k$-tensor on a vector space $V$ is defined as a $k$-linear function
$$
f: V \times \dots \times V \to \mathbb R
$$
A $0$-tensor is simply defined as a scalar in $\mathbb R$.

A tensor is alternating if
$$
f(v_{\sigma(1)}, \dots, v_{\sigma(n)}) = \mathop{\mathrm{sgn}}(\sigma) f(v_1, \dots, v_n)
$$
where $\sigma$ is a permutation.

```

```{definition, , name="Exterior power of vector space"}

Let $V$ be a vector space, then the set of all alternating $k$-tensors of $V$ is denoted with $A_k(V)$
$$
\begin{aligned}
A_0(V) &= \mathbb R \\
A_1(V) &= V^\vee \\
\dots
\end{aligned}
$$

Sometimes we also denote $A_k(V) = \bigwedge^k(V^\vee)$, and refer to the space as the $k$-th exterior
power of $V^\vee$.

```

```{definition, , name="Exterior power of the cotangent bundle"}
The disjoint union of all $k$-th exterior power of all cotangent spaces of a manifold is called the
$k$-th exterior power of the manifold's cotangent bundle.
$$
\sideset{}{^k}\bigwedge(T^*M) = \bigsqcup_{p \in M} \sideset{}{^k}\bigwedge(T_p^*M) \\
$$
```

```{theorem}
At any point $p \in M$, if $(U, x^1, \dots, x^n)$ is a chart about $p$, the
collection is a basis for the vector space $\bigwedge^k(T_p^*M)$
$$
dx^I = dx^{i_1} \wedge \dots \wedge dx^{i_k}
$$
where $I = \{i_1, \dots, i_k\}$ samples from $1, \dots, n$ without replacement.
That is, if $\omega \in \bigwedge^k(T_p^*M)$ then
$$
\alpha = \sum \alpha \left (\frac{\partial}{\partial x^I}\right ) dx^I
$$
where
$$
\frac{\partial}{\partial x^I} = \left (\frac{\partial}{\partial x^{i_1}}, \quad \dots, \quad \frac{\partial}{\partial x^{i_n}} \right )
$$
```


```{proposition}
The $k$-th exterior power of the cotangent bundle can be defined as a smooth manifold in the similar
fashion as tangent bundle.
```

## Differential Forms

```{definition, , name="Differential forms"}
A differential $k$-form
$$
\omega: M \to \sideset{}{^k}\bigwedge(T^*M)
$$
is a section of the vector bundle.
```

```{proposition}

If $\omega$ is a $k$-form defined in a neighborhood of $p$, and written in local coordinates about a point $p$,
$$
\omega = \sum a_I dx^I
$$
then $\omega$ is smooth at $p$ iff all $a^I$ is smooth at $p$.


```

```{definition, , name="Pull back"}

If $F: U \subset M \to N$ is a function defined about $p$, and $\alpha \in \bigwedge^k(T_p^*N)$,
its pull back $F_*\alpha \in \bigwedge^k(T_p^*M)$ is defined as
$$
F^*\alpha(X_1, \dots, X_n) = \alpha(F_*X_1, \dots, F_*X_n)
$$

If $F \in C^\infty_p(M, N)$ is a smooth function, $\omega \in C^\infty(N, \bigwedge^k(T_p^*N))$ is a $k$-form, then its pull back is defined pointwise
$$
(F^*\omega)_p = F^*(\omega_p)
$$
then $F^*\omega_p \in C^\infty(M, \bigwedge^k(T_p^*M))$ (see \@ref(prp:pull-back-char)).

The pull back of a real function $h$ ($0$-form) is the $0$-form
$$
F^*h = h \circ F
$$

```


```{definition, , name="Codifferential"}

If $F \in C^\infty_p(M, N)$, the codifferential is its pull back of a $1$-form, or equivalently, the dual of its
differential, or equivalently,
$$
F^*(\omega)(X) = \omega(F_* X)
$$
```


```{proposition pull-back-char, }
\n

1. If $F \in C^\infty_p(M, N)$, then for any $h \in C^\infty_p(N)$,
    $$
    F^*(dh) = d(F^*h)
    $$
2. If $F \in C^\infty_p(M, N)$, $\omega \in C^\infty_p(M, \bigwedge^r(T^*_M)), \tau \in C^\infty_p(M, \bigwedge^k(T^*_M))$ then their wedge product
    $\omega \wedge \tau \in C^\infty_p(M, \bigwedge^{r + k}(T^*_M))$ and
    $$
    F^*(\omega \wedge \tau) = F^*\omega \wedge F^*\tau
    $$

This proves the pull back of a smooth form is smooth.
```